src/impl/TLS13.Impl.Client.Driver.Receive.fst
@@ -63,14 +63,14 @@ let lemma_receive_observation_network_witness
   (input old_network_out network_out old_app_out app_out:B.bytes)
   : Lemma
       (requires
-        CT.network_bytes_end_to_end_correct
+        CT.coalesced_network_bytes_end_to_end_correct
           st0 st1 buffer_resp input
           old_network_out network_out old_app_out app_out)
       (ensures
         exists st_network st_before observed_input
                observed_old_network_out observed_network_out
                observed_old_app_out observed_app_out.
-          CT.network_bytes_end_to_end_correct
+          CT.coalesced_network_bytes_end_to_end_correct
             st_before
             st_network
             buffer_resp
@@ -85,7 +85,7 @@ let lemma_receive_observation_network_witness
   introduce exists st_network st_before observed_input
                    observed_old_network_out observed_network_out
                    observed_old_app_out observed_app_out.
-      CT.network_bytes_end_to_end_correct
+      CT.coalesced_network_bytes_end_to_end_correct
         st_before
         st_network
         buffer_resp
@@ -105,7 +105,7 @@ let lemma_receive_observation_network_ok
   (input old_network_out network_out old_app_out app_out:B.bytes)
   : Lemma
       (requires
-        CT.network_bytes_end_to_end_correct
+        CT.coalesced_network_bytes_end_to_end_correct
           st0 st1 buffer_resp input
           old_network_out network_out old_app_out app_out)
       (ensures
@@ -124,7 +124,7 @@ let lemma_receive_observation_network_ok
   eliminate exists st_network st_before observed_input
                    observed_old_network_out observed_network_out
                    observed_old_app_out observed_app_out.
-    CT.network_bytes_end_to_end_correct
+    CT.coalesced_network_bytes_end_to_end_correct
       st_before
       st_network
       buffer_resp
@@ -151,7 +151,7 @@ let lemma_receive_observation_network_ok
       exists st_observed st_before' observed_input'
              observed_old_network_out' observed_network_out'
              observed_old_app_out' observed_app_out'.
-        CT.network_bytes_end_to_end_correct
+        CT.coalesced_network_bytes_end_to_end_correct
           st_before'
           st_observed
           buffer_resp
@@ -170,7 +170,7 @@ let lemma_receive_observation_network_ok
       introduce exists st_observed st_before' observed_input'
                        observed_old_network_out' observed_network_out'
                        observed_old_app_out' observed_app_out'.
-        CT.network_bytes_end_to_end_correct
+        CT.coalesced_network_bytes_end_to_end_correct
           st_before'
           st_observed
           buffer_resp
@@ -519,7 +519,7 @@ fn rec receive_application_data
             network.BN.completed_drive_pending_len;
           receive_workflow_response = buffer_resp;
         };
-        assert (pure (CT.network_bytes_end_to_end_correct
+        assert (pure (CT.coalesced_network_bytes_end_to_end_correct
           'st0
           st_network
           buffer_resp
@@ -544,7 +544,7 @@ fn rec receive_application_data
         assert (pure (
           (receive_workflow_observation result)
             .client_receive_observed_response == buffer_resp));
-        assert (pure (CT.network_bytes_end_to_end_correct
+        assert (pure (CT.coalesced_network_bytes_end_to_end_correct
           'st0
           st_network
           (receive_workflow_observation result)
@@ -558,7 +558,7 @@ fn rec receive_application_data
         assert (pure (exists st_observed st_before input
                             old_network_out observed_network_out
                             old_app_out observed_app_out.
-          CT.network_bytes_end_to_end_correct
+          CT.coalesced_network_bytes_end_to_end_correct
             st_before
             st_observed
             (receive_workflow_observation result)
@@ -571,7 +571,7 @@ fn rec receive_application_data
         assert (pure (exists st_observed st_before input
                             old_network_out observed_network_out
                             old_app_out observed_app_out.
-          CT.network_bytes_end_to_end_correct
+          CT.coalesced_network_bytes_end_to_end_correct
             st_before
             st_observed
             (receive_workflow_observation result)
@@ -642,7 +642,7 @@ fn rec receive_application_data
       BS.DriveYield network_result _ _ _ -> {
         let buffer_resp =
           network_result.buffered_network_read.network_read_buffer_resp;
-        assert (pure (CT.network_bytes_end_to_end_correct
+        assert (pure (CT.coalesced_network_bytes_end_to_end_correct
           'st0
           st_network
           buffer_resp
